Stlc/LemmasEvaluation.v
@@ -1,0 +1,31 @@
+Require Export Stlc.SpecSyntax.
+Require Export Stlc.SpecEvaluation.
+Require Export Stlc.LemmasSyntaxBasic.
+
+Lemma evalPlusToStar {t t'} : evalPlus t t' -> evalStar t t'.
+Proof.
+  induction 1; apply rt1n_trans with y; eauto using clos_refl_trans_1n.
+Qed.
+      
+Lemma cycles_dont_terminate_help {t t'} : evalStar t' t -> evalPlus t t -> ~Terminating t'.
+Proof.
+  unfold not.
+  intros tptot ttot term.
+  depind term.
+  depind tptot.
+  * depind ttot.
+    + exact (H1 x H (rt1n_refl Tm eval x)).
+    + refine (H1 y H _). 
+      apply evalPlusToStar; assumption.
+  * apply H1 with y; assumption.
+Qed.
+
+Lemma cycles_dont_terminate {t} : evalPlus t t -> ~Terminating t.
+Proof.
+  apply cycles_dont_terminate_help; constructor.
+Qed.
+
+
+(* Local Variables: *)
+(* coq-load-path: (("." "Stlc")) *)
+(* End: *)
