Stlc/Omega.v
@@ -1,0 +1,34 @@
+Require Export Stlc.SpecSyntax.
+Require Export Stlc.SpecEvaluation.
+Require Export Stlc.SpecTyping.
+Require Export Stlc.LemmasTyping.
+Require Export Stlc.LemmasEvaluation.
+
+Definition stlcOmega (ty : Ty) : Tm := app (fixt tunit ty (abs (tunit ⇒ ty) (var 0))) unit. 
+
+Lemma stlcOmegaT {Γ ty} : ⟪ Γ ⊢ stlcOmega ty : ty ⟫.
+Proof.
+  unfold stlcOmega. crushTyping.
+Qed.
+
+Definition stlcOmegaHelp (ty : Ty) : Tm := app (abs tunit (app (fixt tunit ty (abs (tunit ⇒ ty) (var 0)))[wkl 1] (var 0))) unit.
+
+
+Lemma stlcOmega_cycles {ty} : evalPlus (stlcOmega ty) (stlcOmega ty).
+Proof.
+  apply t1n_trans with (stlcOmegaHelp ty).
+  * unfold stlcOmega, stlcOmegaHelp. refine (eval_ctx (papp₁ phole unit) _ _); constructor.
+  * apply t1n_step.
+    unfold stlcOmega, stlcOmegaHelp.
+    repeat constructor.
+Qed.
+    
+Lemma stlcOmega_div {ty} : ~Terminating (stlcOmega ty).
+Proof.
+  apply cycles_dont_terminate.
+  apply stlcOmega_cycles.
+Qed.
+
+(* Local Variables: *)
+(* coq-load-path: (("." "Stlc")) *)
+(* End: *)
