UVal/UVal.v
@@ -1,0 +1,62 @@
+Require Import Stlc.SpecEvaluation.
+Require Import Stlc.SpecSyntax.
+Require Import Stlc.SpecTyping.
+Require Import Stlc.LemmasTyping.
+Require Import Stlc.LemmasEvaluation.
+
+Fixpoint UVal (n : nat) : Ty :=
+  match n with
+    | 0 => tunit
+    | S n => tunit ⊎ tunit ⊎ tbool ⊎ (UVal n × UVal n) ⊎ (UVal n ⇒ UVal n) ⊎ (UVal n ⊎ UVal n)
+  end.
+
+Fixpoint unkUVal (n : nat) : Tm :=
+  match n with
+    | 0 => unit
+    | S n => inl unit
+  end.
+
+Lemma unkUValT {Γ n} : ⟪ Γ ⊢ unkUVal n : UVal n ⟫.
+Proof.
+  induction n; eauto using Typing.
+Qed.
+
+Definition inUnit (n : nat) : Tm := abs tunit (inr (inl (var 0))).
+
+Lemma inUnitT {Γ n} : ⟪ Γ ⊢ inUnit n : tunit ⇒ UVal (S n) ⟫.
+Proof.
+  unfold inUnit, UVal. crushTyping.
+Qed.
+
+Definition inBool (n : nat) : Tm := abs tbool (inr (inr (inl (var 0)))).
+
+Lemma inBoolT {Γ n} : ⟪ Γ ⊢ inBool n : tbool ⇒ UVal (S n) ⟫.
+Proof.
+  unfold inBool, UVal. crushTyping.
+Qed.
+
+Definition inProd (n : nat) : Tm := abs (UVal n × UVal n) (inr (inr (inr (inl (var 0))))).
+
+Lemma inProd_T {Γ n} : ⟪ Γ ⊢ inProd n : (UVal n × UVal n) ⇒ UVal (S n) ⟫.
+Proof.
+  unfold inProd, UVal. crushTyping.
+Qed.
+
+Definition inArr (n : nat) : Tm := abs (UVal n ⇒ UVal n) (inr (inr (inr (inr (inl (var 0)))))).
+
+Lemma inArr_T {Γ n} : ⟪ Γ ⊢ inArr n : (UVal n ⇒ UVal n) ⇒ UVal (S n) ⟫.
+Proof.
+  unfold inArr, UVal. crushTyping.
+Qed.
+
+Definition inSum (n : nat) : Tm := abs (UVal n ⊎ UVal n) (inr (inr (inr (inr (inr (var 0)))))).
+
+Lemma inSum_T {Γ n} : ⟪ Γ ⊢ inSum n : (UVal n ⊎ UVal n) ⇒ UVal (S n) ⟫.
+Proof.
+  unfold inSum, UVal. crushTyping.
+Qed.
+
+
+(* Local Variables: *)
+(* coq-load-path: (("." "UVal") ("../Stlc" "Stlc")) *)
+(* End: *)
